@prefix srr: <https://w3id.org/srr#> .
@prefix rdf:    <http://www.w3.org/1999/02/22-rdf-syntax-ns#> .
@prefix owl:    <http://www.w3.org/2002/07/owl#> .
@prefix rdfs:   <http://www.w3.org/2000/01/rdf-schema#> .
@prefix xsd:    <http://www.w3.org/2001/XMLSchema#> .
@prefix dcterms: <http://purl.org/dc/terms/> .
@prefix vann:   <http://purl.org/vocab/vann/> .
@prefix voaf: <http://purl.org/vocommons/voaf#> .
@prefix foaf:   <http://xmlns.com/foaf/0.1/> .
@base <https://w3id.org/srr#> .

#################################
# METADATA
#################################

<https://w3id.org/srr#> rdf:type voaf:Vocabulary , 
                                    owl:Ontology ;
    dcterms:title "Structural Reliability Representation"@en ;
    dcterms:creator [rdf:type foaf:Person ; foaf:name "Lini Xiang" ] ;
    dcterms:description "This ontology includes two reliability analysis methods, Monte Carlo  and First Order Second Moment. It can be combined with other building ontology to form a wider range of structure department ontology."@en ;
    dcterms:license "http://creativecommons.org/licenses/by/2.0" ;
    vann:preferredNamespacePrefix "srr" ;
    vann:preferredNamespaceUri "https://w3id.org/srr#" ;

#################################
# CLASSES
#################################

srr:StructuralSystem 
              a owl:Class ;
              rdfs:comment """The structural system represents an abstract representation of the mechanical concepts of civil,  mechanical or hydraulic or aerospace engineering."""@en ;
              rdfs:label "Structural System"@en .

srr:RandomVariable 
              a owl:Class ;
              rdfs:subClassOf srr:StructuralSystem ;
              rdfs:comment """Random variables are used for structural uncertainty analysis. It refers to events that may or may not occur in reality, and therefore have random and uncertain values."""@en ;
              rdfs:label "RandomVariable"@en .

srr:Distribution 
              a owl:Class ;
              rdfs:subClassOf srr:RandomVariable ;
              rdfs:comment """Distribution is a statistical feature that describes the value of a random variable."""@en ;
              rdfs:label "Distribution"@en .

srr:Mean 
              a owl:Class ;
              rdfs:subClassOf srr:RandomVariable ;
              rdfs:comment """The mean value of the distribution of a random variable."""@en ;
              rdfs:label "Mean"@en .

srr:StandardDeviation 
              a owl:Class ;
              rdfs:subClassOf srr:RandomVariable ;
              rdfs:comment """Standard deviation describes the volatility of the distribution of a random variable."""@en ;
              rdfs:label "Standard Deviation"@en .

srr:LimitEquation 
              a owl:Class ;
              rdfs:subClassOf srr:StructuralSystem ;
              rdfs:comment """The limit state equation is the relationship between variables when the structure is about to crack."""@en ;
              rdfs:label "Limit Equation"@en .

srr:MenteCarlo 
              a owl:Class ;
              rdfs:subClassOf srr:LimitEquation ;
              rdfs:comment """The Monte Carlo method simulates the approximate solution of the problem through the statistical results of random sampling."""@en ;
              rdfs:label "Mente Carlo Method"@en .

srr:Sample 
              a owl:Class ;
	      rdfs:subClassOf srr:MenteCarlo ;
              rdfs:comment """The sampling results of Monte Carlo method."""@en ;
              rdfs:label "Sample"@en .

srr:FailureSum 
              a owl:Class ;
	      rdfs:subClassOf srr:MenteCarlo ;
              rdfs:comment """This is the total number of structural failures after substituting the sample into the limit state function."""@en ; 
              rdfs:label "Failure Sum"@en .

srr:Reliability 
              a owl:Class ;
              rdfs:comment """It is an important design index that enables the reliability of the building structure to meet various predetermined functions."""@en ;
              rdfs:label "Reliability"@en .

srr:FailureProbability 
              a owl:Class ;
              rdfs:comment """The possibility of structural damage during the service period."""@en ;
	      rdfs:label "Failure Probability"@en .

srr:FOSM 
              a owl:Class ;
              rdfs:subClassOf srr:LimitEquation ;
              rdfs:comment """The first order second moment method is to use the mean value and standard deviation to perform linear Taylor expansion of the limit function, to solve the problem iteratively ."""@en ;
              rdfs:label "FOSM"@en .
			  
srr:Gradient  
              a owl:Class ;
              rdfs:subClassOf srr:FOSM ;
              rdfs:comment """The function changes fastest in this direction."""@en ;
              rdfs:label "Gradient"@en .

srr:InitialValue 
              a owl:Class ;
	      rdfs:subClassOf srr:FOSM ;
              rdfs:comment """The starting point of executing the first order second moment method."""@en ;
              rdfs:label "Initial Value"@en .

srr:BreakPoint 
              a owl:Class ;
              rdfs:subClassOf srr:FOSM ;
              rdfs:comment """Most likely point of failure."""@en ;
              rdfs:label "Break Point"@en .

#################################
# OBJECT PROPERTIES
#################################

srr:hasMechanicalCharacteristics 
              a owl:ObjectProperty ;
              rdfs:domain owl:Class ;
              rdfs:range  rdfs:Resource ;
              rdfs:comment """A relationship that various mechanical properties exist within a structural system."""@en ;
              rdfs:label "has Mechanical Characteristics"@en .

srr:hasStatisticsCharacteristics 
              a owl:ObjectProperty ;
              rdfs:domain owl:Class ;
              rdfs:range  rdfs:Resource ;
              rdfs:comment """There are statistics relevant quantities that can describe things."""@en ;
              rdfs:label "has Statistics Characteristics"@en .

srr:hasSolutions 
              a owl:ObjectProperty ;
              rdfs:domain owl:Class ;
              rdfs:range  rdfs:Resource ;
              rdfs:comment """Defines that the function has a method to obtain solution."""@en ;
              rdfs:label "has Solutions"@en .

srr:hasStepsWithinSolutions 
              a owl:ObjectProperty ;
              rdfs:domain owl:Class ;
              rdfs:range  rdfs:Resource ;
              rdfs:comment """Describes that there are many steps within the solution."""@en ;
              rdfs:label "has Steps Within Solutions"@en .

srr:hasCalculation 
              a owl:ObjectProperty ;
              rdfs:domain owl:Class ;
              rdfs:range  rdfs:Resource ;
              rdfs:comment """Describes the mathematical process of transforming one quantity to another."""@en ;
              rdfs:label "has Calculation"@en .

#################################################################
#    Data properties
#################################################################

srr:hasNumericalValue 
              a owl:DatatypeProperty ;
              rdfs:domain owl:Class ;
              rdfs:range  xsd:Double ;
              rdfs:comment """Describes a physical quantity that has a numerical value."""@en ;
              rdfs:label "has Numerical Value"@en .

srr:noNumericalValue 
              a owl:DatatypeProperty ;
              rdfs:domain owl:Class ;
              rdfs:range  xsd:string ;
              rdfs:comment """Describes a physical quantity that does not have the usual mathematical value in numerical form."""@en ;
              rdfs:label "no Numerical Value"@en .

